lib/zoo_parabs/vertex.mli
@@ -7,6 +7,8 @@ val get_task :
   t -> bool Pool.task
 val set_task :
   t -> bool Pool.task -> unit
+val set_task' :
+  t -> unit Pool.task -> unit
 
 val precede :
   t -> t -> unit
